Prove lemmas about LawfulMemUpdate

src/ReactorModel/Objects/Reactor/Theorems/LawfulUpdate.lean
@@ -9,13 +9,26 @@ theorem UniqueIDs.updated [ReactorType.WellFounded α] {rtr₁ rtr₂ : α}
       |>.trans (Equivalent.from_lawfulUpdate u m₂).symm 
       |>.to_eq
 
-def LawfulMemUpdate.member [ReactorType α] {rtr₁ rtr₂ : α}
-    (u : LawfulMemUpdate cpt i f rtr₁ rtr₂) : Member cpt i rtr₁ :=
-  sorry
+def LawfulMemUpdate.member [ReactorType α] {rtr₁ rtr₂ : α} :
+    (LawfulMemUpdate cpt i f rtr₁ rtr₂) → Member cpt i rtr₁
+  | final _ h _  => .final $ Partial.mem_iff.mpr ⟨_, h⟩ 
+  | nest _ h _ u => .nest h u.member
 
-def LawfulMemUpdate.unique [Indexable α] {rtr rtr₁ rtr₂ : α}
-    (u₁ : LawfulMemUpdate cpt i f rtr rtr₁) (u₂ : LawfulMemUpdate cpt i f rtr rtr₂) : rtr₁ = rtr₂ := 
-  sorry 
+open Indexable in
+theorem LawfulMemUpdate.unique [Indexable α] {rtr rtr₁ rtr₂ : α}
+    (u₁ : LawfulMemUpdate cpt i f rtr rtr₁) (u₂ : LawfulMemUpdate cpt i f rtr rtr₂) : rtr₁ = rtr₂ := by
+  induction u₁ generalizing rtr₂ <;> cases u₂
+  case final.final e₁ h₁ h₁' _ h₂ h₂' e₂ =>
+    injection h₁ ▸ h₂ with h
+    exact RootEqualUpTo.ext (RootEqualUpTo.trans e₁.symm e₂) (h₂' ▸ h ▸ h₁')
+  case nest.nest j₁ _ _ _ _ e₁ h₁ h₁' u₁ hi j₂ _ _ u₂ h₂ h₂' e₂ =>
+    have h : j₁ = j₂ := by injection unique_ids.allEq (u₁.member.nest h₁) (u₂.member.nest h₂)
+    subst h; cases h₁ ▸ h₂; cases hi u₂
+    exact RootEqualUpTo.ext (RootEqualUpTo.trans e₁.symm e₂) $ h₁' ▸ h₂'.symm
+  case final.nest h₁ _ _ _ _ u h₂ _ _ =>
+    exact nomatch unique_ids.allEq (Member.final $ Partial.mem_iff.mpr ⟨_, h₁⟩) (u.member.nest h₂)
+  case nest.final h₁ _ u _ _ h₂ _ _ =>
+    exact nomatch unique_ids.allEq (Member.final $ Partial.mem_iff.mpr ⟨_, h₂⟩) (u.member.nest h₁)
 
 theorem LawfulMemUpdate.ne_comm [Indexable α] {rtr rtr₁ rtr₁' rtr₂ rtr₂' : α} 
     (u₁ : LawfulMemUpdate cpt₁ i₁ f₁ rtr rtr₁) (u₂ : LawfulMemUpdate cpt₂ i₂ f₂ rtr₁ rtr₂) 
